disj/PathSplits.v
@@ -4,8 +4,8 @@ Theorem lc_join_split `{redCFG} t1 t2 (p q1 q2 s : Lab) (i j1 j2 k : Tag)
         (* it is important to cons qj's in front of the t's *)
         (Hlc : last_common ((q1,j1) :: t1) ((q2,j2) :: t2) (s,k))
         (Hneq : q1 <> q2)
-        (Hpath1 : TPath (root,start_tag) (p,i) ((p,i) :<: (q1,j1) :< t1))
-        (Hpath2 : TPath (root,start_tag) (p,i) ((p,i) :<: (q2,j2) :< t2))
+        (Hpath1 : TPath (root,start_tag) (p,i) ((p,i) :: (q1,j1) :: t1))
+        (Hpath2 : TPath (root,start_tag) (p,i) ((p,i) :: (q2,j2) :: t2))
   : exists qq qq', (s,qq,qq') ∈ splits p.
 Proof.
 Admitted.
